theories/L6_PCPS/inline_letapp.v
@@ -1,0 +1,1043 @@
+From compcert.lib Require Import Coqlib.
+Require Import L6.tactics.
+From CertiCoq.L6 Require Import cps ctx Ensembles_util List_util functions map_util identifiers cps_util stemctx
+     rename logical_relations alpha_conv eval functions.
+From Coq Require Import Arith.Arith NArith.BinNat Strings.String Lists.List
+     omega.Omega Sets.Ensembles Relations.Relation_Operators Classes.Morphisms.
+From MetaCoq.Template Require Import BasicAst. (* For identifier names *)
+Require Import ExtLib.Structures.Monad ExtLib.Structures.MonadState ExtLib.Data.Monads.StateMonad.
+
+Import MonadNotation.
+Open Scope monad_scope.
+Open Scope ctx_scope.
+
+Fixpoint inline_letapp
+         (e : exp) (* function body to be inlined *)
+         (z : var) (* the binding used for the app *)
+  : option (exp_ctx * var) := (* Returns an evaluation context that computes the result of the function and puts it in the variable that's returned *)
+  match e with
+  | Econstr x ct xs e =>
+    res <- inline_letapp e z ;;
+    let (C, v) := (res : exp_ctx * var) in
+    ret (Econstr_c x ct xs C, v)
+  | Ecase _ _ =>
+    (* currently we don't support inlining of let-bound applications of functions that
+         are not straight line code *)
+    None
+  | Eproj x n ct y e =>
+    res <- inline_letapp e z ;;
+    let (C, v) := (res : exp_ctx * var) in
+    ret (Eproj_c x n ct y C, v)
+  | Eletapp x f ft ys e =>
+    res <- inline_letapp e z ;;
+    let (C, v) := (res : exp_ctx * var) in
+    ret (Eletapp_c x f ft ys C, v)
+  | Efun B e =>      
+    res <- inline_letapp e z ;;
+    let (C, v) := (res : exp_ctx * var) in
+    ret (Efun1_c B C, v)
+  | Eapp f ft ys =>
+    ret (Eletapp_c z f ft ys Hole_c, z)
+  | Eprim x p ys e  =>
+    res <- inline_letapp e z ;;
+    let (C, v) := (res : exp_ctx * var) in      
+    ret (Eprim_c x p ys C, v)
+  | Ehalt x => ret (Hole_c, x)
+  end.
+
+
+Lemma bound_var_inline_letapp x e C x' :
+  inline_letapp e x = Some (C, x') ->
+  bound_var_ctx C \subset x |: bound_var e.
+Proof. 
+  revert C.
+  induction e using exp_ind'; simpl; intros C Hin;
+    (try match goal with
+         | [ _ : context[inline_letapp ?E ?X] |- _ ] =>
+           destruct (inline_letapp E X) as [[C' z] | ] eqn:Hin'; inv Hin
+         end);
+    (try now (normalize_bound_var; normalize_bound_var_ctx;
+              eapply Union_Included; sets; eapply Included_trans;
+              [ eapply IHe; reflexivity | ]; sets)).
+  congruence.  
+  inv Hin. normalize_bound_var. repeat normalize_bound_var_ctx. sets.
+  inv Hin. normalize_bound_var. repeat normalize_bound_var_ctx. sets.
+Qed.
+
+
+(* TODO move *)
+Lemma bound_var_occurs_free_Eletapp_Included x f t ys e :
+  Included _ (Union _ (bound_var e) (occurs_free e))
+           (Union _ (bound_var (Eletapp x f t ys e))
+                  (occurs_free (Eletapp x f t ys e))).
+Proof with eauto with Ensembles_DB.
+  repeat normalize_bound_var. repeat normalize_occurs_free.
+  rewrite <- Union_assoc.
+  apply Included_Union_compat...
+  eapply Included_trans. now apply occurs_free_Eletapp_Included with (ft := t).
+  normalize_occurs_free...
+Qed.
+
+Lemma inline_letapp_var_eq x e C x' :
+  inline_letapp e x = Some (C, x') ->
+  x' = x \/ x' \in bound_var e :|: occurs_free e.
+Proof.
+  revert C. induction e using exp_ind'; simpl; intros C Hin;
+              (try match goal with
+                   | [ _ : context[inline_letapp ?E ?X] |- _ ] =>
+                     destruct (inline_letapp E X) as [[C' z] | ] eqn:Hin'; inv Hin
+                   end).
+  - destruct (IHe C' eq_refl); eauto. right. 
+    eapply bound_var_occurs_free_Econstr_Included; eauto.
+  - congruence.
+  - destruct (IHe C' eq_refl); eauto. right. 
+    eapply bound_var_occurs_free_Eproj_Included; eauto.
+  - destruct (IHe C' eq_refl); eauto. right. 
+    eapply bound_var_occurs_free_Eletapp_Included; eauto.
+  - destruct (IHe C' eq_refl); eauto. right. 
+    eapply bound_var_occurs_free_Efun_Included; eauto.
+  - inv Hin. eauto.
+  - destruct (IHe C' eq_refl); eauto. right. 
+    eapply bound_var_occurs_free_Eprim_Included; eauto.
+  - inv Hin. normalize_occurs_free. sets.
+Qed.
+
+Lemma occurs_fee_inline_letapp C e x x' e' :
+  inline_letapp e x = Some (C, x') ->
+  occurs_free (C |[ e' ]|)  \subset occurs_free e :|: (occurs_free e' \\ bound_stem_ctx C).
+Proof.
+  revert C x x' e'; induction e; intros C x x' e' Hin; simpl in Hin;
+    (try match goal with
+         | [ _ : context [inline_letapp ?E ?X ] |- _] => destruct (inline_letapp E X) as [[C' x''] | ] eqn:Hin'; inv Hin
+         end); try congruence.
+  - simpl. repeat normalize_occurs_free.
+    eapply Union_Included; sets.
+    eapply Setminus_Included_Included_Union. eapply Included_trans.
+    eapply IHe; eauto. normalize_bound_stem_ctx. rewrite <- Setminus_Union.
+    rewrite <- !Union_assoc. rewrite <- Union_Setminus; tci.
+    rewrite <- Union_Included_Union_Setminus with (s3 := [set v]); tci; sets. 
+  - simpl. repeat normalize_occurs_free.
+    eapply Union_Included; sets.
+    eapply Setminus_Included_Included_Union. eapply Included_trans.
+    eapply IHe; eauto. normalize_bound_stem_ctx. rewrite <- Setminus_Union.
+    rewrite <- !Union_assoc. rewrite <- Union_Setminus; tci.
+    rewrite <- Union_Included_Union_Setminus with (s3 := [set v]); tci; sets. 
+  - simpl. repeat normalize_occurs_free.
+    eapply Union_Included; sets.
+    eapply Setminus_Included_Included_Union. eapply Included_trans.
+    eapply IHe; eauto. normalize_bound_stem_ctx. rewrite <- Setminus_Union.
+    rewrite <- !Union_assoc. rewrite <- Union_Setminus; tci.
+    rewrite <- Union_Included_Union_Setminus with (s3 := [set v]); tci; sets. 
+  - simpl. repeat normalize_occurs_free.
+    eapply Union_Included; sets.
+    eapply Setminus_Included_Included_Union. eapply Included_trans.
+    eapply IHe; eauto. normalize_bound_stem_ctx. rewrite (Union_commut (name_in_fundefs f)).      
+    rewrite <- Setminus_Union.
+    rewrite <- !Union_assoc. rewrite <- Union_Setminus; tci.
+    rewrite <- Union_Included_Union_Setminus with (s3 := name_in_fundefs f); tci; sets. 
+  - inv Hin. simpl. repeat normalize_occurs_free. repeat normalize_bound_stem_ctx.
+    xsets.
+  - simpl. repeat normalize_occurs_free.
+    eapply Union_Included; sets.
+    eapply Setminus_Included_Included_Union. eapply Included_trans.
+    eapply IHe; eauto. normalize_bound_stem_ctx. rewrite <- Setminus_Union.
+    rewrite <- !Union_assoc. rewrite <- Union_Setminus; tci.
+    rewrite <- Union_Included_Union_Setminus with (s3 := [set v]); tci; sets.
+  - inv Hin. repeat normalize_occurs_free. repeat normalize_bound_stem_ctx.
+    simpl. sets. 
+Qed.
+
+
+Lemma unique_bindings_inline_letapp C e x x' : 
+  inline_letapp e x = Some (C, x') ->
+  ~ x \in bound_var e ->
+  unique_bindings e ->
+  unique_bindings_c C.
+Proof.
+  revert C x x'; induction e; intros C x x' Hin Hbv Hub; simpl in Hin;
+    (try match goal with
+         | [ _ : context [inline_letapp ?E ?X ] |- _] => destruct (inline_letapp E X) as [[C' x''] | ] eqn:Hin'; inv Hin
+         end); try congruence.
+  - inv Hub. constructor; eauto. intros Hc; eapply H1.
+    eapply bound_var_inline_letapp in Hc; eauto. inv Hc; eauto. inv H.
+    exfalso. eapply Hbv; eauto.
+    eapply IHe; eauto.
+  - inv Hub. constructor; eauto. intros Hc; eapply H1.
+    eapply bound_var_inline_letapp in Hc; eauto. inv Hc; eauto. inv H.
+    exfalso. eapply Hbv; eauto.
+    eapply IHe; eauto.
+  - inv Hub. constructor; eauto. intros Hc; eapply H1.
+    eapply bound_var_inline_letapp in Hc; eauto. inv Hc; eauto. inv H.
+    exfalso. eapply Hbv; eauto.
+    eapply IHe; eauto.
+  - inv Hub. constructor; eauto.
+    eapply IHe; eauto.
+    eapply Disjoint_Included_l.
+    eapply bound_var_inline_letapp. eassumption.
+    eapply Union_Disjoint_l; sets. eapply Disjoint_Singleton_l.
+    intros Hc. eapply Hbv; eauto.
+  - inv Hin. constructor; eauto.
+    intros Hc; inv Hc.
+    constructor. 
+  - inv Hub. constructor; eauto. intros Hc; eapply H1.
+    eapply bound_var_inline_letapp in Hc; eauto. inv Hc; eauto. inv H.
+    exfalso. eapply Hbv; eauto.
+    eapply IHe; eauto.
+  - inv Hin. constructor.
+Qed.
+
+Lemma bound_stem_inline_letapp x e C x' :
+  inline_letapp e x = Some (C, x') ->
+  bound_stem_ctx C \subset x |: bound_var e.
+Proof. 
+  revert C. induction e using exp_ind'; simpl; intros C Hin;
+              (try match goal with
+                   | [ _ : context[inline_letapp ?E ?X] |- _ ] =>
+                     destruct (inline_letapp E X) as [[C' z] | ] eqn:Hin'; inv Hin
+                   end);
+              (try now (normalize_bound_var; normalize_bound_stem_ctx;
+                        eapply Union_Included; sets; eapply Included_trans;
+                        [ eapply IHe; reflexivity | ]; sets)).
+  congruence.
+
+  normalize_bound_var; normalize_bound_stem_ctx. eapply Union_Included.
+  eapply Included_trans. eapply name_in_fundefs_bound_var_fundefs. now sets.
+  eapply Included_trans. eapply IHe. reflexivity. sets.
+
+  inv Hin. normalize_bound_var. repeat normalize_bound_stem_ctx. sets.
+  inv Hin. normalize_bound_var. repeat normalize_bound_stem_ctx. sets.
+Qed.
+
+
+Lemma inline_letapp_var_eq_alt x e C x' :
+  inline_letapp e x = Some (C, x') ->
+  (x' = x /\ x \in bound_stem_ctx C) \/ x' \in bound_stem_ctx C :|: occurs_free e.
+Proof.
+  revert C. induction e using exp_ind'; simpl; intros C Hin;
+              (try match goal with
+                   | [ _ : context[inline_letapp ?E ?X] |- _ ] =>
+                     destruct (inline_letapp E X) as [[C' z] | ] eqn:Hin'; inv Hin
+                   end).
+  - destruct (IHe C' eq_refl); eauto. right.
+    inv H. now left; eauto.
+    normalize_occurs_free. normalize_bound_stem_ctx.
+    rewrite !Union_assoc, Union_Setminus_Included; tci; sets. inv H; eauto. 
+  - congruence.
+  - destruct (IHe C' eq_refl); eauto. right.
+    inv H. now left; eauto.
+    normalize_occurs_free. normalize_bound_stem_ctx. inv H; eauto.
+    rewrite !Union_assoc. rewrite Union_Setminus_Included with (s3 := [set v]); tci. sets.
+  - destruct (IHe C' eq_refl); eauto. right.
+    inv H. now left; eauto.
+    normalize_occurs_free. normalize_bound_stem_ctx.
+    rewrite !Union_assoc, Union_Setminus_Included; tci; sets. inv H; eauto 20.
+  - destruct (IHe C' eq_refl); eauto. right.
+    inv H. now left; eauto.
+    normalize_occurs_free. normalize_bound_stem_ctx.
+    rewrite !Union_assoc, Union_Setminus_Included; tci; sets. inv H; eauto. 
+  - inv Hin. eauto.
+  - destruct (IHe C' eq_refl); eauto. right.
+    inv H. now left; eauto.
+    normalize_occurs_free. normalize_bound_stem_ctx.
+    rewrite !Union_assoc, Union_Setminus_Included; tci; sets. inv H; eauto.
+  - inv Hin. normalize_occurs_free; sets.
+Qed.
+
+
+Ltac dec_vars :=
+  repeat match goal with
+         | [ H: (if var_dec ?X ?Y then _ else _) = 0 |- _] =>
+           destruct (var_dec X Y); try inversion H; pi0
+         end.
+
+
+Lemma num_occur_inline_letapp e f C x x' :
+  num_occur e f 0 ->
+  inline_letapp e  x = Some (C, x') ->
+  x <> f ->
+  num_occur_ec C f 0 /\ x' <> f. 
+Proof.
+  revert f C x x'.
+  induction e using exp_ind'; intros g C y x' Hnum  Hin Hneq; simpl in Hin;
+    (try match goal with
+         | [ _ : context [inline_letapp ?E ?X ] |- _] => destruct (inline_letapp E X) as [[C' x''] | ] eqn:Hin'; inv Hin
+         end); try congruence.
+  - inv Hnum. pi0. eapply IHe in H4; eauto. destructAll. split; eauto.
+    rewrite plus_comm. constructor. eassumption.
+  - inv Hnum. pi0. eapply IHe in H5; [| eassumption |]; eauto. destructAll. split; eauto.
+    constructor. eassumption.
+  - inv Hnum. pi0. eapply IHe in H5; [| eassumption |]; eauto. destructAll. split; eauto.
+    constructor. eassumption.   
+  - inv Hnum. pi0. eapply IHe in Hin'; try eassumption; eauto. destructAll. split; eauto.
+    constructor; eassumption.
+  - Opaque num_occur_list. inv Hin. inv Hnum. split; eauto.
+    replace (num_occur_list (v :: l) g) with (num_occur_list (v :: l) g + 0) by omega.
+    econstructor. eauto. econstructor.
+  - inv Hnum. pi0. eapply IHe in H4; eauto. destructAll. split; eauto.
+    rewrite plus_comm. constructor. eassumption.
+  - inv Hin. inv Hnum. 
+    Transparent num_occur_list.
+    simpl in *.
+    destruct (cps_util.var_dec g x'); subst; try congruence. split; eauto. econstructor. 
+Qed.
+
+Lemma num_occur_inline_letapp_leq e f C x x' m :
+  num_occur e f m ->
+  inline_letapp e  x = Some (C, x') ->
+  exists n, num_occur_ec C f n /\ n <= m.
+Proof.
+  revert m f C x x'. induction e using exp_ind'; intros m g C y x' Hnum  Hin; simpl in Hin;
+                       (try match goal with
+                            | [ _ : context [inline_letapp ?E ?X ] |- _] => destruct (inline_letapp E X) as [[C' x''] | ] eqn:Hin'; inv Hin
+                            end); try congruence.
+  - inv Hnum. eapply IHe in Hin'; eauto. destructAll.
+    eexists; split. econstructor. eassumption. omega.
+  - inv Hnum. eapply IHe in Hin'; eauto. destructAll.
+    eexists; split. econstructor. eassumption. omega.
+  - inv Hnum. eapply IHe in Hin'; eauto. destructAll.
+    eexists; split. econstructor. eassumption. omega.
+  - inv Hnum. eapply IHe in Hin'; eauto. destructAll.
+    eexists; split. econstructor. eassumption. eassumption. omega.
+  - inv Hnum. inv Hin. eexists; split. econstructor. now constructor. omega.
+  - inv Hnum. eapply IHe in Hin'; eauto. destructAll.
+    eexists; split. econstructor. eassumption. omega.
+  - inv Hin. eexists. split. constructor. omega.
+Qed.
+
+Lemma inline_letapp_var_num_occur x e C x' :
+  inline_letapp e x = Some (C, x') ->
+  x' = x \/ (exists m, m > 0 /\ num_occur e x' m).
+Proof.
+  revert C. induction e using exp_ind'; simpl; intros C Hin;
+              (try match goal with
+                   | [ _ : context[inline_letapp ?E ?X] |- _ ] =>
+                     destruct (inline_letapp E X) as [[C' z] | ] eqn:Hin'; inv Hin
+                   end);
+              try now (destruct (IHe C' eq_refl); eauto; destructAll; right;
+                       eauto; eexists; split; [| econstructor; eassumption ]; omega).
+  - congruence.
+  - destruct (IHe C' eq_refl); eauto. right. destructAll.
+    edestruct (proj2 (e_num_occur_mut x')). 
+    eexists. constructor. 2:{ econstructor; eauto. }
+    omega.
+  - inv Hin. now left.
+  - inv Hin. right. eauto. eexists. split. 2:{ econstructor. }
+    simpl. rewrite peq_true. omega.
+Qed.
+
+Lemma inline_letapp_None e x sig :
+  inline_letapp e x = None ->
+  inline_letapp (rename_all_ns sig e) x = None.
+Proof.
+  revert x sig; induction e; intros x sig Hinl; simpl in *;
+    try match goal with
+        | [H : context[inline_letapp ?E ?X] |- _ ] => destruct (inline_letapp E X) as [[C' y] | ] eqn:Hinl'; inv Hinl
+        end;
+    try now (erewrite IHe; [| eassumption ]).
+  - reflexivity.
+  - inv Hinl.
+  - inv Hinl.
+Qed.
+
+Lemma inline_letapp_var_eq_alt' x e C x' :
+  inline_letapp e x = Some (C, x') ->
+  (x' = x /\ x \in bound_stem_ctx C) \/ x' \in bound_var e :|: occurs_free e.
+Proof.
+  revert C. induction e using exp_ind'; simpl; intros C Hin;
+              (try match goal with
+                   | [ _ : context[inline_letapp ?E ?X] |- _ ] =>
+                     destruct (inline_letapp E X) as [[C' z] | ] eqn:Hin'; inv Hin
+                   end).
+  - destruct (IHe C' eq_refl); eauto. now inv H; eauto.
+    normalize_occurs_free. normalize_bound_var.
+    rewrite !Union_assoc, Union_Setminus_Included; tci; sets. inv H; eauto. 
+  - congruence.
+  - destruct (IHe C' eq_refl); eauto.
+    inv H. now left; eauto.
+    normalize_occurs_free. normalize_bound_var. inv H; eauto.
+    rewrite !Union_assoc. rewrite Union_Setminus_Included with (s3 := [set v]); tci. sets.
+  - destruct (IHe C' eq_refl); eauto.
+    inv H. now left; eauto.
+    normalize_occurs_free. normalize_bound_var.
+    rewrite !Union_assoc, Union_Setminus_Included; tci; sets. inv H; eauto 20.
+  - destruct (IHe C' eq_refl); eauto. 
+    inv H. now left; eauto.
+    normalize_occurs_free. normalize_bound_var.
+    rewrite !Union_assoc, Union_Setminus_Included; tci; sets. inv H; eauto.
+    eapply Included_trans. eapply name_in_fundefs_bound_var_fundefs. sets.
+  - inv Hin. eauto.
+  - destruct (IHe C' eq_refl); eauto.
+    inv H. now left; eauto.
+    normalize_occurs_free. normalize_bound_var.
+    rewrite !Union_assoc, Union_Setminus_Included; tci; sets. inv H; eauto.
+  - inv Hin. normalize_occurs_free; sets.
+Qed.
+
+(* TODO move *)
+Lemma num_occur_ec_eq C x m n :
+  num_occur_ec C x m ->
+  n = m ->
+  num_occur_ec C x n.
+Proof. intros; subst; eauto. Qed.
+
+Lemma num_occur_eq C x m n :
+  num_occur C x m ->
+  n = m ->
+  num_occur C x n.
+Proof. intros; subst; eauto. Qed.
+
+Lemma inline_letapp_gt_zero e v C x :
+  inline_letapp e v = Some (C, x) ->
+  v <> x ->
+  exists m, m > 0 /\ num_occur e x m.
+Proof. 
+  revert C.
+  induction e using exp_ind'; intros C Hin Hneq; simpl in Hin;
+    (try match goal with
+         | [ _ : context [inline_letapp ?E ?X ] |- _] => destruct (inline_letapp E X) as [[C' x''] | ] eqn:Hin'; inv Hin
+         end); try congruence; try (edestruct IHe; eauto; destructAll);
+      (try now eexists; split; [| eapply num_occur_eq; econstructor; eauto ]; omega).
+  - edestruct e_num_occur_fds. eexists. split. 2:{ eapply num_occur_eq. constructor; eassumption. reflexivity. }
+    omega.
+  - eexists. split. 2:{ constructor. }
+    inv Hin. simpl. rewrite peq_true. omega.
+Qed.
+
+Lemma inline_letapp_num_occur e v C x z n :
+  inline_letapp e v = Some (C, x) ->
+  v <> z ->
+  num_occur e z n ->    
+  if (var_dec z x) then num_occur_ec C z (n - 1) else num_occur_ec C z n.
+Proof.
+  revert C n.
+  induction e using exp_ind'; intros C (* m Hleq *) m Hin Hneq Hnum; simpl in Hin;
+    (try match goal with
+         | [ _ : context [inline_letapp ?E ?X ] |- _] => destruct (inline_letapp E X) as [[C' x''] | ] eqn:Hin'; inv Hin
+         end); try congruence; inv Hnum; destruct (var_dec z x); subst;
+      (try now eapply num_occur_ec_eq; [ constructor; eapply IHe; eauto | omega ]);
+      (try now edestruct inline_letapp_gt_zero; [ eassumption | eassumption | ]; destructAll;
+       match goal with
+       | [H1 : num_occur _ _ _, H2 : num_occur _ _ _ |- _ ] => eapply num_occur_det in H1; [| eapply H2 ]; subst
+       end;
+       eapply num_occur_ec_eq; [ constructor; eapply IHe; eauto | omega ]).
+  - edestruct inline_letapp_gt_zero; [ eassumption | eassumption | ]; destructAll.
+    match goal with
+    | [H1 : num_occur _ _ _, H2 : num_occur _ _ _ |- _ ] => eapply num_occur_det in H1; [| eapply H2 ]; subst
+    end.
+    eapply num_occur_ec_eq. constructor. eapply IHe; eauto. eassumption. omega .
+  - eapply num_occur_ec_eq. constructor. eapply IHe; eauto. eassumption. omega .
+  - inv Hin. contradiction.
+  - inv Hin. eapply num_occur_ec_eq. econstructor. now constructor. omega.
+  - inv Hin. eapply num_occur_ec_eq. econstructor. simpl. rewrite peq_true. omega.
+  - inv Hin. eapply num_occur_ec_eq. econstructor. simpl. rewrite peq_false; eauto.
+Qed. 
+
+
+
+
+
+
+
+Definition remove_steps_letapp cenv (P1 P2 P3 : PostT) :=
+             forall (x f : positive) (t : fun_tag) (ys : list map_util.M.elt) (e1 : exp)
+                    (rho1 : map_util.M.t val)
+                    (xs : list var) (e_b1 : exp) (v1 : val) (e2 e2' e_b2: exp) (rho2 rho2' rhoc2  rhoc1 : M.t val) 
+                    (fl : fundefs) (h : var) (vs : list val) (rhoc1' : map_util.M.t val) (c1 c1' c2 c2' : nat),
+               rho1 ! f = Some (Vfun rhoc1 fl h) ->
+               get_list ys rho1 = Some vs ->
+               find_def h fl = Some (t, xs, e_b1) ->
+               set_lists xs vs (def_funs fl fl rhoc1 rhoc1) = Some rhoc1' ->
+               bstep_fuel cenv rhoc1' e_b1 (Res v1) c1 ->
+
+               P1 (e_b1, rhoc1', c1) (e_b2, rhoc2, c2) ->
+               P2 (e1, M.set x v1 rho1, c1') (e2', rho2', c2') ->
+               P3 (Eletapp x f t ys e1, rho1, c1 + c1' + cost (Eletapp x f t ys e1))
+                  (e2, rho2, c2 + c2').
+
+Definition remove_steps_letapp' cenv (P1 P2 P3 : PostT) :=
+  forall (x f : positive) (t : fun_tag) (ys : list map_util.M.elt) (e1 : exp)
+         (rho1 : map_util.M.t val)
+         (xs : list var) (e_b1 : exp) (v1 : val) (e2 e2' e_b2: exp) (rho2 rho2' rhoc2  rhoc1 : M.t val) 
+         (fl : fundefs) (h : var) (vs : list val) (rhoc1' : map_util.M.t val) (c1 c1' c2 c2' : nat),
+    rho1 ! f = Some (Vfun rhoc1 fl h) ->
+    get_list ys rho1 = Some vs ->
+    find_def h fl = Some (t, xs, e_b1) ->
+    set_lists xs vs (def_funs fl fl rhoc1 rhoc1) = Some rhoc1' ->
+    bstep_fuel cenv rhoc1' e_b1 (Res v1) c1 ->
+    
+    P1 (e_b1, rhoc1', c1) (e_b2, rhoc2, c2 + 1) ->
+    P2 (e1, M.set x v1 rho1, c1') (e2', rho2', c2') ->
+    P3 (Eletapp x f t ys e1, rho1, c1 + c1' + cost (Eletapp x f t ys e1)) (e2, rho2, c2 + c2'). 
+
+
+Definition remove_steps_letapp_OOT cenv (P1 P2 : PostT) :=
+  forall (x x' f : positive) (t : fun_tag) (ys : list map_util.M.elt) (e1 : exp) (rho1 : map_util.M.t val)
+         (xs : list var) (e_b1 : exp) (r : res) (e2 e_b2 : exp) (rho2 rhoc1 : M.t val) (rhoc2 : env) 
+         (fl : fundefs) (h : var) (vs : list val) (rhoc1' : map_util.M.t val) (c1 c2 : nat),
+    rho1 ! f = Some (Vfun rhoc1 fl h) ->
+    get_list ys rho1 = Some vs ->
+    find_def h fl = Some (t, xs, e_b1) ->
+    set_lists xs vs (def_funs fl fl rhoc1 rhoc1) = Some rhoc1' ->
+    bstep_fuel cenv rhoc1' e_b1 r c1 ->
+    
+    P1 (e_b1, rhoc1', c1) (e_b2, rhoc2, c2) ->
+    P2 (Eletapp x f t ys e1, rho1, c1 + cost (Eletapp x' f t ys e1)) (e2, rho2, c2 ). 
+
+Definition remove_steps_letapp_OOT' cenv (P1 P2 : PostT) :=
+
+  forall (x f : positive) (t : fun_tag) (ys : list map_util.M.elt) (e1 : exp) (rho1 : map_util.M.t val)
+         (xs : list var) (e_b1 : exp) (r : res) (e2 e_b2 : exp) (rho2 rhoc1 : M.t val) (rhoc2 : env) 
+         (fl : fundefs) (h : var) (vs : list val) (rhoc1' : map_util.M.t val) (c1 c2 : nat),
+    rho1 ! f = Some (Vfun rhoc1 fl h) ->
+    get_list ys rho1 = Some vs ->
+    find_def h fl = Some (t, xs, e_b1) ->
+    set_lists xs vs (def_funs fl fl rhoc1 rhoc1) = Some rhoc1' ->
+    bstep_fuel cenv rhoc1' e_b1 r c1 ->
+    
+    P1 (e_b1, rhoc1', c1) (e_b2, rhoc2, c2) ->
+    P2 (Eletapp x f t ys e1, rho1, c1 + cost (Eletapp x f t ys e1)) (e2, rho2, c2 - 1). 
+
+
+Section Inline_correct.
+
+  Context (cenv : ctor_env) (P1  : PostT) (PG : PostGT). 
+
+  Context (Hless_steps_letapp : remove_steps_letapp cenv P1 P1 P1)
+          (Hless_steps_letapp' : remove_steps_letapp' cenv P1 P1 P1)
+          (Hless_steps_letapp_OOT : remove_steps_letapp_OOT cenv P1 P1)
+          (Hless_steps_letapp_OOT' : remove_steps_letapp_OOT' cenv P1 P1)
+          (Hpost_zero : forall e rho, post_zero e rho P1).
+  
+  Lemma inline_letapp_correct k x sig f t ys e1 e2 e' C C' x' rho1 rho2 : 
+    (forall m rhoc rhoc' B f' xs vs e,
+        m < k -> 
+        M.get f rho1 = Some (Vfun rhoc B f') ->
+        find_def f' B = Some (t, xs, e) ->
+        get_list ys rho1 = Some vs ->
+        set_lists xs vs (def_funs B B rhoc rhoc) = Some rhoc' ->
+        preord_exp cenv P1 PG m (e, rhoc') (C' |[ e' ]|, rho2)) ->
+
+    (forall m rho1' rho2' rhoc B f' t xs e,
+        m < k ->
+        M.get f rho1 = Some (Vfun rhoc B f') ->
+        find_def f' B = Some (t, xs, e) -> length xs = length ys ->
+        preord_env_P_inj cenv PG (occurs_free e1) m (sig {x ~> x'}) rho1' rho2' ->
+        preord_exp cenv P1 PG m (e1, rho1') (e2, rho2')) ->
+
+    preord_env_P_inj cenv PG (occurs_free (Eletapp x f t ys e1)) k sig rho1 rho2 ->
+    
+    Disjoint _ (bound_var_ctx C' :|: bound_var_ctx C) (image sig (occurs_free e1 \\ [set x])) ->    
+    ~ x \in (image sig (occurs_free e1 \\ [set x])) ->
+    interprable C' = true ->
+    inline_letapp e' x = Some (C, x') ->
+    
+    preord_exp cenv P1 PG k (Eletapp x f t ys e1, rho1) (C' |[ C |[ e2 ]| ]|, rho2).
+  Proof.
+    revert C' k x sig f t ys e1 e2 C x' rho1 rho2; induction e';
+      intros C' k x sig f' t ys e1 e2 C x' rho1 rho2 Hyp1 Hyp2 Hpre Hdis Him Hint Hin; simpl in Hin;
+        try match goal with
+        | [ _ : context [inline_letapp ?E ?X] |- _ ] =>
+          (destruct (inline_letapp E X) as [ [C'' u] | ] eqn:Hin'; simpl in Hin; inv Hin)
+        end.
+    - intros r1 c2 Hleq Hs1. inv Hs1.
+      + exists OOT, 0. split; [| split ]; eauto. constructor. eapply cost_gt_0.
+        eapply Hpost_zero; eauto. now simpl; eauto.
+      + edestruct (IHe' (comp_ctx_f C' (Econstr_c v c l Hole_c)) k) with (C := C'') as [r2 [c2' [Hs2 [Hp2 Hv2]]]].
+        9:{ econstructor 2; eauto. }
+        * rewrite <- app_ctx_f_fuse. simpl ( _ |[ _ ]|). eapply Hyp1.
+        * eapply Hyp2.
+        * eassumption.
+        * destruct  bound_var_ctx_comp_ctx as [Heq1 _ ]. rewrite Heq1.
+          rewrite bound_var_Econstr_c, bound_var_Hole_c in *. xsets. 
+        * eassumption.
+        * eapply interprable_comp_f_l; eauto.
+        * eassumption.
+        * eassumption. 
+        * rewrite <- app_ctx_f_fuse in *. simpl in *. do 2 eexists. 
+          split; [| split ]. eassumption. eassumption. eassumption.
+    - inv Hin.
+    - intros r1 c2 Hleq Hs1. inv Hs1.
+      + exists OOT, 0. split; [| split ]; eauto. constructor. eapply cost_gt_0.
+        now eapply Hpost_zero; eauto. now simpl; eauto.
+      + edestruct (IHe' (comp_ctx_f C' (Eproj_c v c n v0 Hole_c)) k) with (C := C'') as [r2 [c2' [Hs2 [Hp2 Hv2]]]].
+        9:{ econstructor 2; eauto. }
+        * rewrite <- app_ctx_f_fuse. simpl ( _ |[ _ ]|). eapply Hyp1.
+        * eapply Hyp2.
+        * eassumption.
+        * destruct  bound_var_ctx_comp_ctx as [Heq1 _ ]. rewrite Heq1.
+          rewrite bound_var_Eproj_c, bound_var_Hole_c in *. xsets. 
+        * eassumption.
+        * eapply interprable_comp_f_l; eauto.
+        * eassumption.
+        * eassumption. 
+        * rewrite <- app_ctx_f_fuse in *. simpl in *. do 2 eexists.
+          split; [| split ]. eassumption. eassumption. eassumption. 
+    - intros r1 c2 Hleq Hs1. inv Hs1.
+      + exists OOT, 0. split; [| split ]; eauto. constructor. eapply cost_gt_0.
+        now eapply Hpost_zero; eauto. now simpl; eauto.
+      + edestruct (IHe' (comp_ctx_f C' (Eletapp_c v v0 f l Hole_c)) k) with (C := C'') as [r2 [c2' [Hs2 [Hp2 Hv2]]]].
+        9:{ econstructor 2; eauto. }
+        * rewrite <- app_ctx_f_fuse. simpl ( _ |[ _ ]|). eapply Hyp1.
+        * eapply Hyp2.
+        * eassumption.
+        * destruct  bound_var_ctx_comp_ctx as [Heq1 _ ]. rewrite Heq1.
+          rewrite bound_var_Eletapp_c, bound_var_Hole_c in *. xsets. 
+        * eassumption.
+        * eapply interprable_comp_f_l; eauto.
+        * eassumption.
+        * eassumption. 
+        * rewrite <- app_ctx_f_fuse in *. simpl in *. do 2 eexists.
+          split; [| split ]. eassumption. eassumption. eassumption.
+    - intros r1 c2 Hleq Hs1. inv Hs1.
+      + exists OOT, 0. split; [| split ]; eauto. constructor. eapply cost_gt_0.
+        now eapply Hpost_zero; eauto. now simpl; eauto.
+      + edestruct (IHe' (comp_ctx_f C' (Efun1_c f  Hole_c)) k) with (C := C'') as [r2 [c2' [Hs2 [Hp2 Hv2]]]].
+        9:{ econstructor 2; eauto. }
+        * rewrite <- app_ctx_f_fuse. simpl ( _ |[ _ ]|). eapply Hyp1.
+        * eapply Hyp2. 
+        * eassumption.
+        * destruct  bound_var_ctx_comp_ctx as [Heq1 _ ]. rewrite Heq1.
+          rewrite bound_var_Fun1_c, bound_var_Hole_c in *. xsets. 
+        * eassumption.
+        * eapply interprable_comp_f_l; eauto.
+        * eassumption.
+        * eassumption. 
+        * rewrite <- app_ctx_f_fuse in *. simpl in *. do 2 eexists.
+          split; [| split ]. eassumption. eassumption. eassumption.
+    - inv Hin. simpl (_ |[ _ ]|).
+      intros r1 c2 Hleq Hs1. inv Hs1.
+      + exists OOT, 0. split; [| split ]; eauto. constructor. eapply cost_gt_0.
+        now eapply Hpost_zero; eauto. now simpl; eauto.
+      + inv H0.  
+
+        * edestruct (Hyp1 (k -1)) as [r2 [c2' [Hs2 [Hp2 Hv2]]]]; [ | | | | | | now eapply H13 | ]; eauto.
+          simpl in *; omega. simpl in *; omega.
+          destruct r2; [ simpl in Hv2; contradiction | ].
+          eapply interpret_ctx_bstep_l in Hs2; [| eassumption ].
+          destruct Hs2 as (rho2' & n1 & n2 & Hadd & Hctx & Heval); subst.
+          inv Heval.
+          edestruct (Hyp2 (k - 1 - cin1)) with (rho2' := M.set x' v1 rho2') as [r3 [c3 [Hs3 [Hp3 Hv3]]]];
+            [ | |  | | | | now eapply H14 | ]; eauto. 
+          simpl in *; omega.  
+          rewrite (get_list_length_eq _ _ _ H10). eapply set_lists_length_eq. now eauto. 
+          
+          { eapply preord_env_P_inj_set_alt; [| eassumption | eassumption ].
+            eapply preord_env_P_inj_eq_env_P; [| eapply eq_env_P_refl | ].
+            2:{ eapply interpret_ctx_eq_env_P. eassumption. sets. }
+            eapply preord_env_P_inj_antimon.
+            eapply preord_env_P_inj_monotonic; [| eassumption ]. omega. normalize_occurs_free. sets.  } 
+            
+          simpl in *; omega.
+          inv H1. 
+          exists r3, (n1 + (n2 + c3)).
+          split. eapply interpret_ctx_bstep_r. eassumption.
+          constructor 2.
+          2:{ simpl; replace (n2 + c3 - S (Datatypes.length l))
+                      with (n2 - cost (Eapp v f l) + c3) by (simpl in *; omega).
+              econstructor; eauto. } simpl in *; omega.
+          split.
+
+          assert (Heq : c2 = cin1 + cin2 + S (Datatypes.length ys)).
+          { rewrite <- (NPeano.Nat.sub_add (S (Datatypes.length ys)) c2). rewrite H6. reflexivity.
+            eassumption. } rewrite Heq. 
+          rewrite plus_assoc.
+          now eapply Hless_steps_letapp; eauto. 
+          eapply preord_res_monotonic. eassumption. simpl in *; omega.
+        * edestruct (Hyp1 (k -1)) as [r2 [c2' [Hs2 [Hp2 Hv2]]]]; [ | | | | | | now eapply H13 | ]; eauto.
+          simpl in *; omega. simpl in *; omega.
+          destruct r2; [ | simpl in Hv2; contradiction ].
+
+          eexists OOT, c2'. split; [| split ]. 
+
+          eapply eval_ctx_app_OOT_Eapp. eassumption. eassumption.
+
+          replace c2 with (c2 - cost (Eletapp x' f' t ys e1) + cost (Eletapp x' f' t ys e1)) by (simpl in *; omega). 
+          now eapply Hless_steps_letapp_OOT; eauto. 
+          simpl; eauto. 
+    - intros r1 c2 Hleq Hs1. inv Hs1.
+      + exists OOT, 0. split; [| split ]; eauto. constructor. eapply cost_gt_0.
+        now eapply Hpost_zero; eauto. now simpl; eauto.
+      + inv H0.
+        
+        * edestruct (Hyp1 (k -1)) as [r2 [c2' [Hs2 [Hp2 Hv2]]]]; [ | | | | | | now eapply H13 | ]; eauto.
+          simpl in *; omega. simpl in *; omega.
+          destruct r2; [ simpl in Hv2; contradiction | ].
+          eapply interpret_ctx_bstep_l in Hs2; [| eassumption ].
+          destruct Hs2 as (rho2' & n1 & n2 & Hadd & Hctx & Heval); subst.
+          inv Heval. inv H1.
+        * edestruct (Hyp1 (k -1)) as [r2 [c2' [Hs2 [Hp2 Hv2]]]]; [ | | | | | | now eapply H13 | ]; eauto.
+          simpl in *; omega. simpl in *; omega.
+          destruct r2; [ | simpl in Hv2; contradiction ].
+
+          eexists OOT, c2'. split; [| split ]. 
+
+          eapply eval_ctx_app_OOT_Eprim. eassumption. eassumption.          
+
+          replace c2 with (c2 - cost (Eletapp x f' t ys e1) + cost (Eletapp x f' t ys e1)) by (simpl in *; omega). 
+          now eapply Hless_steps_letapp_OOT; eauto. 
+          simpl; eauto. 
+    - inv Hin. simpl (_ |[ _ ]|). 
+      intros r1 c2 Hleq Hs1. inv Hs1.
+      + exists OOT, 0. split; [| split ]; eauto. constructor. eapply cost_gt_0.
+        now eapply Hpost_zero; eauto. now simpl; eauto.
+      + inv H0.
+
+        * edestruct (Hyp1 (k -1)) as [r2 [c2' [Hs2 [Hp2 Hv2]]]]; [ | | | | | | now eapply H13 | ]; eauto.
+          simpl in *; omega. simpl in *; omega.
+          destruct r2; [ simpl in Hv2; contradiction | ].
+          eapply interpret_ctx_bstep_l in Hs2; [| eassumption ].
+          destruct Hs2 as (rho2' & n1 & n2 & Hadd & Hctx & Heval); subst.
+          inv Heval. inv H1. assert (Heq : n2 = 1) by (simpl in *; omega). subst. 
+          edestruct (Hyp2 (k - 1 - cin1)) with (rho2' := rho2') as [r3 [c3 [Hs3 [Hp3 Hv3]]]];
+            [ | | | | | | now eapply H14 | ]; eauto.
+          simpl in *; omega.
+          
+          rewrite (get_list_length_eq _ _ _ H10). eapply set_lists_length_eq. now eauto. 
+
+          { eapply preord_env_P_inj_set_l; [| eassumption | eassumption ].
+            eapply preord_env_P_inj_eq_env_P; [| eapply eq_env_P_refl | ].
+            2:{ eapply interpret_ctx_eq_env_P. eassumption. sets. }
+            eapply preord_env_P_inj_antimon.
+            eapply preord_env_P_inj_monotonic; [| eassumption ]. omega. normalize_occurs_free. sets. } 
+
+          simpl in *; omega.
+          do 2 eexists. split. eapply interpret_ctx_bstep_r. eassumption. eassumption.
+
+          split. 
+          assert (Heq : c2 = cin1 + cin2 + S (Datatypes.length ys)).
+          { rewrite <- (NPeano.Nat.sub_add (S (Datatypes.length ys)) c2). rewrite H6. reflexivity.
+            eassumption. } rewrite Heq. 
+          now eapply Hless_steps_letapp'; eauto. 
+          eapply preord_res_monotonic. eassumption. simpl in *; omega.
+
+        * edestruct (Hyp1 (k -1)) as [r2 [c2' [Hs2 [Hp2 Hv2]]]]; [ | | | | | | now eapply H13 | ]; eauto.
+          simpl in *; omega. simpl in *; omega.
+          destruct r2; [ | simpl in Hv2; contradiction ].
+
+          eexists OOT, (c2' - 1). split; [| split ]. 
+
+          eapply bstep_fuel_OOT_monotonic. eapply eval_ctx_app_OOT_Ehalt. eassumption. eassumption. omega.
+
+          replace c2 with (c2 - cost (Eletapp x f' t ys e1) + cost (Eletapp x f' t ys e1)) by (simpl in *; omega). 
+          now eapply Hless_steps_letapp_OOT'; eauto.
+          simpl; eauto. 
+  Qed.
+
+
+  Lemma eq_env_P_def_funs_not_in_P_r' (B B' : fundefs) (P : Ensemble M.elt) 
+        (rho : cps.M.t val) (rho1 rho2 : M.t val) : 
+    eq_env_P P rho1 (def_funs B' B rho rho2) ->
+    Disjoint M.elt P (name_in_fundefs B) ->
+    eq_env_P P rho1 rho2.
+  Proof.
+    intros H1 Hdis x Hin. assert (Hin' := Hin). eapply H1 in Hin.
+    destruct (Decidable_name_in_fundefs B). destruct (Dec x).
+    - exfalso. eapply Hdis. constructor; eassumption.
+    - rewrite def_funs_neq in Hin ; eauto.
+  Qed.
+
+  (* TOPO move to eval.v *)
+  Lemma interpret_ctx_fuel_env_eq_P S C rho rho' n :    
+    interpret_ctx_fuel cenv C rho (Res rho') n ->
+    Disjoint _ (bound_var_ctx C) S ->
+    eq_env_P S rho rho'.
+  Proof.
+    revert rho rho' n. induction C; intros rho rho' i Hi Hd.
+    - inv Hi. inv H0. eapply eq_env_P_refl.
+    - inv Hi. inv H0.
+      normalize_bound_var_ctx_in_ctx. eapply IHC in H9; [| now sets ].
+      eapply eq_env_P_set_not_in_P_l'. eassumption. sets.
+    - inv Hi. inv H0.
+      normalize_bound_var_ctx_in_ctx. eapply IHC in H11; [| now sets ].
+      eapply eq_env_P_set_not_in_P_l'. eassumption. sets.
+    - inv Hi. inv H0.
+    - inv Hi. inv H0.
+      normalize_bound_var_ctx_in_ctx. eapply IHC in H14; [| now sets ].
+      eapply eq_env_P_set_not_in_P_l'. eassumption. sets.
+    - inv Hi. inv H0.
+    - inv Hi. inv H0.
+      normalize_bound_var_ctx_in_ctx. eapply IHC in H6; [| now sets ].
+      eapply eq_env_P_sym in H6. eapply eq_env_P_def_funs_not_in_P_r' in H6. eapply eq_env_P_sym. eassumption.
+      eapply Disjoint_Included_r. eapply name_in_fundefs_bound_var_fundefs. sets.
+    - inv Hi. inv H0.
+  Qed.
+
+
+  (* Lemma preord_env_P_inj_set_alt' (S : Ensemble var) (rho1 rho2 : env)  *)
+  (*       (k : nat) f (x y : var) (v1 v2 : val) :  *)
+  (*   preord_env_P_inj cenv PG (S \\ [set x]) k f rho1 rho2 -> *)
+  (*   preord_val cenv PG k v1 v2 -> *)
+  (*   f x = y -> *)
+  (*   (* ~ In _ (image f (Dom_map rho1)) y -> *) *)
+  (*   preord_env_P_inj cenv PG S k (f {x ~> y}) (M.set x v1 rho1) (M.set y v2 rho2). *)
+  (* Proof. *)
+  (*   intros Henv Hv Heq z HP. unfold extend.  *)
+  (*   destruct (peq z x) as [| Hneq]. *)
+  (*   - subst. intros z Hget. *)
+  (*     rewrite M.gss in Hget. inv Hget. eexists. rewrite M.gss; eauto. *)
+  (*   - intros z' Hget. rewrite M.gso in Hget; eauto.  *)
+  (*     destruct (peq (f z) y). *)
+  (*     + exfalso. eapply Hnin. eexists; eauto. *)
+  (*       split; eauto. eexists; eauto. *)
+  (*     + edestruct (Henv z); eauto. *)
+  (*       constructor; eauto. intros Hc. inv Hc. congruence.  *)
+  (*       eexists. rewrite M.gso; eauto.  *)
+  (* Qed. *)
+
+
+  Lemma inline_letapp_correct_alt k x z sig f t ys e1 e2 e' C C' x' rho1 rho2 : 
+    (forall m rhoc rhoc' B f' xs vs e,
+        m < k -> 
+        M.get f rho1 = Some (Vfun rhoc B f') ->
+        find_def f' B = Some (t, xs, e) ->
+        get_list ys rho1 = Some vs ->
+        set_lists xs vs (def_funs B B rhoc rhoc) = Some rhoc' ->
+        preord_exp cenv P1 PG m (e, rhoc') (C' |[ e' ]|, rho2)) ->
+
+    (forall m rho1' rho2' rhoc B f' t xs e,
+        m < k ->
+        M.get f rho1 = Some (Vfun rhoc B f') ->
+        find_def f' B = Some (t, xs, e) -> length xs = length ys ->
+        eq_env_P (Complement _ [set x]) rho1 rho1' ->
+        eq_env_P (Complement _ (bound_var e' :|: bound_var_ctx C') \\ [set x']) rho2 rho2' ->
+        Dom_map rho1' <--> x |: Dom_map rho1 ->
+        preord_env_P_inj cenv PG (occurs_free e1) m (sig {x ~> x'}) rho1' rho2' ->
+        preord_exp cenv P1 PG m (e1, rho1') (e2, rho2')) ->
+
+    preord_env_P_inj cenv PG (occurs_free (Eletapp x f t ys e1)) k sig rho1 rho2 ->
+    
+    Disjoint _ (bound_var_ctx C' :|: bound_var_ctx C) (image sig (occurs_free e1 \\ [set x])) ->
+    ~ z \in (image sig (Dom_map rho1)) ->
+            
+    interprable C' = true ->
+    inline_letapp e' z = Some (C, x') ->
+    
+    preord_exp cenv P1 PG k (Eletapp x f t ys e1, rho1) (C' |[ C |[ e2 ]| ]|, rho2).
+  Proof.
+    revert C' k x sig f t ys e1 e2 C x' rho1 rho2; induction e';
+      intros C' k x sig f' t ys e1 e2 C x' rho1 rho2 Hyp1 Hyp2 Hpre Hdis Hnin Hint Hin; simpl in Hin;
+        try match goal with
+        | [ _ : context [inline_letapp ?E ?X] |- _ ] =>
+          (destruct (inline_letapp E X) as [ [C'' u] | ] eqn:Hin'; simpl in Hin; inv Hin)
+        end.
+    - intros r1 c2 Hleq Hs1. inv Hs1.
+      + exists OOT, 0. split; [| split ]; eauto. constructor. eapply cost_gt_0.
+        eapply Hpost_zero; eauto. now simpl; eauto.
+      + edestruct (IHe' (comp_ctx_f C' (Econstr_c v c l Hole_c)) k) with (C := C'') as [r2 [c2' [Hs2 [Hp2 Hv2]]]].
+        9:{ econstructor 2; eauto. }
+        * rewrite <- app_ctx_f_fuse. simpl ( _ |[ _ ]|). eapply Hyp1.
+        * intros. eapply Hyp2; eauto. eapply eq_env_P_antimon. eassumption.
+          eapply Included_Setminus_compat. eapply Complement_antimon. normalize_bound_var; sets.
+          rewrite (proj1 bound_var_ctx_comp_ctx). repeat normalize_bound_var_ctx. sets.
+          reflexivity.
+        * eassumption.
+        * destruct  bound_var_ctx_comp_ctx as [Heq1 _ ]. rewrite Heq1.
+          rewrite bound_var_Econstr_c, bound_var_Hole_c in *. normalize_sets.
+          eapply Disjoint_Included; [| | eapply Hdis]; sets.
+        * eassumption.
+        * eapply interprable_comp_f_l; eauto.
+        * reflexivity.
+        * eassumption. 
+        * rewrite <- app_ctx_f_fuse in *. simpl in *. do 2 eexists. 
+          split; [| split ]. eassumption. eassumption. eassumption.
+    - inv Hin.
+    - intros r1 c2 Hleq Hs1. inv Hs1.
+      + exists OOT, 0. split; [| split ]; eauto. constructor. eapply cost_gt_0.
+        now eapply Hpost_zero; eauto. now simpl; eauto.
+      + edestruct (IHe' (comp_ctx_f C' (Eproj_c v c n v0 Hole_c)) k) with (C := C'') as [r2 [c2' [Hs2 [Hp2 Hv2]]]].
+        9:{ econstructor 2; eauto. }
+        * rewrite <- app_ctx_f_fuse. simpl ( _ |[ _ ]|). eapply Hyp1.
+        * intros. eapply Hyp2; eauto. eapply eq_env_P_antimon. eassumption.
+          eapply Included_Setminus_compat. eapply Complement_antimon. normalize_bound_var; sets.
+          rewrite (proj1 bound_var_ctx_comp_ctx). repeat normalize_bound_var_ctx. sets.
+          reflexivity.
+        * eassumption.
+        * destruct  bound_var_ctx_comp_ctx as [Heq1 _ ]. rewrite Heq1.
+          rewrite bound_var_Eproj_c, bound_var_Hole_c in *.
+          eapply Disjoint_Included; [| | eapply Hdis]; sets.
+        * eassumption.
+        * eapply interprable_comp_f_l; eauto.
+        * reflexivity.
+        * eassumption. 
+        * rewrite <- app_ctx_f_fuse in *. simpl in *. do 2 eexists.
+          split; [| split ]. eassumption. eassumption. eassumption. 
+    - intros r1 c2 Hleq Hs1. inv Hs1.
+      + exists OOT, 0. split; [| split ]; eauto. constructor. eapply cost_gt_0.
+        now eapply Hpost_zero; eauto. now simpl; eauto.
+      + edestruct (IHe' (comp_ctx_f C' (Eletapp_c v v0 f l Hole_c)) k) with (C := C'') as [r2 [c2' [Hs2 [Hp2 Hv2]]]].
+        9:{ econstructor 2; eauto. }
+        * rewrite <- app_ctx_f_fuse. simpl ( _ |[ _ ]|). eapply Hyp1.
+        * intros. eapply Hyp2; eauto. eapply eq_env_P_antimon. eassumption.
+          eapply Included_Setminus_compat. eapply Complement_antimon. normalize_bound_var; sets.
+          rewrite (proj1 bound_var_ctx_comp_ctx). repeat normalize_bound_var_ctx. sets.
+          reflexivity.
+        * eassumption.
+        * destruct  bound_var_ctx_comp_ctx as [Heq1 _ ]. rewrite Heq1.
+          rewrite bound_var_Eletapp_c, bound_var_Hole_c in *. xsets.
+        * eassumption.
+        * eapply interprable_comp_f_l; eauto.
+        * reflexivity.
+        * eassumption. 
+        * rewrite <- app_ctx_f_fuse in *. simpl in *. do 2 eexists.
+          split; [| split ]. eassumption. eassumption. eassumption.
+    - intros r1 c2 Hleq Hs1. inv Hs1.
+      + exists OOT, 0. split; [| split ]; eauto. constructor. eapply cost_gt_0.
+        now eapply Hpost_zero; eauto. now simpl; eauto.
+      + edestruct (IHe' (comp_ctx_f C' (Efun1_c f  Hole_c)) k) with (C := C'') as [r2 [c2' [Hs2 [Hp2 Hv2]]]].
+        9:{ econstructor 2; eauto. }
+        * rewrite <- app_ctx_f_fuse. simpl ( _ |[ _ ]|). eapply Hyp1.
+        * intros. eapply Hyp2; eauto. eapply eq_env_P_antimon. eassumption.
+          eapply Included_Setminus_compat. eapply Complement_antimon. normalize_bound_var; sets.
+          rewrite (proj1 bound_var_ctx_comp_ctx). repeat normalize_bound_var_ctx. sets.
+          reflexivity.          
+        * eassumption.
+        * destruct  bound_var_ctx_comp_ctx as [Heq1 _ ]. rewrite Heq1.
+          rewrite bound_var_Fun1_c, bound_var_Hole_c in *. xsets.
+        * eassumption.
+        * eapply interprable_comp_f_l; eauto.
+        * reflexivity.
+        * eassumption. 
+        * rewrite <- app_ctx_f_fuse in *. simpl in *. do 2 eexists.
+          split; [| split ]. eassumption. eassumption. eassumption.
+    - inv Hin. simpl (_ |[ _ ]|). 
+      intros r1 c2 Hleq Hs1. inv Hs1.
+      + exists OOT, 0. split; [| split ]; eauto. constructor. eapply cost_gt_0.
+        now eapply Hpost_zero; eauto. now simpl; eauto.
+      + inv H0.  
+
+        * edestruct (Hyp1 (k -1)) as [r2 [c2' [Hs2 [Hp2 Hv2]]]]; [ | | | | | | now eapply H13 | ]; eauto.
+          simpl in *; omega. simpl in *; omega.
+          destruct r2; [ simpl in Hv2; contradiction | ].
+          eapply interpret_ctx_bstep_l in Hs2; [| eassumption ].
+          destruct Hs2 as (rho2' & n1 & n2 & Hadd & Hctx & Heval); subst.
+          inv Heval.
+          edestruct (Hyp2 (k - 1 - cin1)) with (rho2' := M.set x' v1 rho2') as [r3 [c3 [Hs3 [Hp3 Hv3]]]];
+            [ | | | | | | | | | now eapply H14 | ]; eauto. 
+          simpl in *; omega.  
+          rewrite (get_list_length_eq _ _ _ H10). eapply set_lists_length_eq. now eauto. 
+
+          eapply eq_env_P_sym. eapply eq_env_P_set_not_in_P_l. eapply eq_env_P_refl. now eauto.
+          eapply eq_env_P_sym. eapply eq_env_P_set_not_in_P_l. eapply eq_env_P_sym.
+          eapply interpret_ctx_fuel_env_eq_P. eassumption.
+          eapply Disjoint_Included_r. eapply Setminus_Included.
+          eapply Disjoint_sym. eapply Complement_Disjoint. now sets.
+          intros Hc. inv Hc. now eauto.
+          
+          rewrite Dom_map_set. reflexivity.
+          
+          { eapply preord_env_P_inj_set_alt'; [| eassumption | eassumption ].
+            eapply preord_env_P_inj_eq_env_P; [| eapply eq_env_P_refl | ].
+            2:{ eapply interpret_ctx_eq_env_P. eassumption. sets. }
+            eapply preord_env_P_inj_antimon.
+            eapply preord_env_P_inj_monotonic; [| eassumption ]. omega. normalize_occurs_free. sets.  }
+            
+          simpl in *; omega.
+          inv H1. 
+          exists r3, (n1 + (n2 + c3)).
+          split. eapply interpret_ctx_bstep_r. eassumption.
+          constructor 2.
+          2:{ simpl; replace (n2 + c3 - S (Datatypes.length l))
+                      with (n2 - cost (Eapp v f l) + c3) by (simpl in *; omega).
+              econstructor; eauto. } simpl in *; omega.
+          split.
+
+          assert (Heq : c2 = cin1 + cin2 + S (Datatypes.length ys)).
+          { rewrite <- (NPeano.Nat.sub_add (S (Datatypes.length ys)) c2). rewrite H6. reflexivity.
+            eassumption. } rewrite Heq. 
+          rewrite plus_assoc.
+          now eapply Hless_steps_letapp; eauto. 
+          eapply preord_res_monotonic. eassumption. simpl in *; omega.
+        * edestruct (Hyp1 (k -1)) as [r2 [c2' [Hs2 [Hp2 Hv2]]]]; [ | | | | | | now eapply H13 | ]; eauto.
+          simpl in *; omega. simpl in *; omega.
+          destruct r2; [ | simpl in Hv2; contradiction ].
+
+          eexists OOT, c2'. split; [| split ]. 
+
+          eapply eval_ctx_app_OOT_Eapp. eassumption. eassumption.
+
+          replace c2 with (c2 - cost (Eletapp x' f' t ys e1) + cost (Eletapp x' f' t ys e1)) by (simpl in *; omega). 
+          now eapply Hless_steps_letapp_OOT; eauto. 
+          simpl; eauto. 
+    - intros r1 c2 Hleq Hs1. inv Hs1.
+      + exists OOT, 0. split; [| split ]; eauto. constructor. eapply cost_gt_0.
+        now eapply Hpost_zero; eauto. now simpl; eauto.
+      + inv H0.
+        
+        * edestruct (Hyp1 (k -1)) as [r2 [c2' [Hs2 [Hp2 Hv2]]]]; [ | | | | | | now eapply H13 | ]; eauto.
+          simpl in *; omega. simpl in *; omega.
+          destruct r2; [ simpl in Hv2; contradiction | ].
+          eapply interpret_ctx_bstep_l in Hs2; [| eassumption ].
+          destruct Hs2 as (rho2' & n1 & n2 & Hadd & Hctx & Heval); subst.
+          inv Heval. inv H1.
+        * edestruct (Hyp1 (k -1)) as [r2 [c2' [Hs2 [Hp2 Hv2]]]]; [ | | | | | | now eapply H13 | ]; eauto.
+          simpl in *; omega. simpl in *; omega.
+          destruct r2; [ | simpl in Hv2; contradiction ].
+
+          eexists OOT, c2'. split; [| split ]. 
+
+          eapply eval_ctx_app_OOT_Eprim. eassumption. eassumption.          
+
+          replace c2 with (c2 - cost (Eletapp x f' t ys e1) + cost (Eletapp x f' t ys e1)) by (simpl in *; omega). 
+          now eapply Hless_steps_letapp_OOT; eauto. 
+          simpl; eauto. 
+    - inv Hin. simpl (_ |[ _ ]|). 
+      intros r1 c2 Hleq Hs1. inv Hs1.
+      + exists OOT, 0. split; [| split ]; eauto. constructor. eapply cost_gt_0.
+        now eapply Hpost_zero; eauto. now simpl; eauto.
+      + inv H0.
+
+        * edestruct (Hyp1 (k -1)) as [r2 [c2' [Hs2 [Hp2 Hv2]]]]; [ | | | | | | now eapply H13 | ]; eauto.
+          simpl in *; omega. simpl in *; omega.
+          destruct r2; [ simpl in Hv2; contradiction | ].
+          eapply interpret_ctx_bstep_l in Hs2; [| eassumption ].
+          destruct Hs2 as (rho2' & n1 & n2 & Hadd & Hctx & Heval); subst.
+          inv Heval. inv H1. assert (Heq : n2 = 1) by (simpl in *; omega). subst. 
+          edestruct (Hyp2 (k - 1 - cin1)) with (rho2' := rho2') as [r3 [c3 [Hs3 [Hp3 Hv3]]]];
+            [ | | | | | | | | | now eapply H14 | ]; eauto.
+          simpl in *; omega.
+          
+          rewrite (get_list_length_eq _ _ _ H10). eapply set_lists_length_eq. now eauto. 
+
+          eapply eq_env_P_sym. eapply eq_env_P_set_not_in_P_l. eapply eq_env_P_refl. now eauto.
+
+          eapply interpret_ctx_fuel_env_eq_P. eassumption. normalize_bound_var. sets. simpl.
+
+          eapply Disjoint_Included_r. eapply Setminus_Included.
+          eapply Disjoint_sym. eapply Complement_Disjoint. now sets.
+
+          rewrite Dom_map_set. reflexivity.
+
+          
+          { eapply preord_env_P_inj_set_l; [| eassumption | eassumption ]. SearchAbout rho2'.
+            eapply preord_env_P_inj_eq_env_P; [| eapply eq_env_P_refl | ].
+            2:{ eapply interpret_ctx_eq_env_P. eassumption. sets. }
+            eapply preord_env_P_inj_antimon.
+            eapply preord_env_P_inj_monotonic; [| eassumption ]. omega. normalize_occurs_free. sets. } 
+
+          simpl in *; omega.
+          do 2 eexists. split. eapply interpret_ctx_bstep_r. eassumption. eassumption.
+
+          split. 
+          assert (Heq : c2 = cin1 + cin2 + S (Datatypes.length ys)).
+          { rewrite <- (NPeano.Nat.sub_add (S (Datatypes.length ys)) c2). rewrite H6. reflexivity.
+            eassumption. } rewrite Heq. 
+          now eapply Hless_steps_letapp'; eauto. 
+          eapply preord_res_monotonic. eassumption. simpl in *; omega.
+
+        * edestruct (Hyp1 (k -1)) as [r2 [c2' [Hs2 [Hp2 Hv2]]]]; [ | | | | | | now eapply H13 | ]; eauto.
+          simpl in *; omega. simpl in *; omega.
+          destruct r2; [ | simpl in Hv2; contradiction ].
+
+          eexists OOT, (c2' - 1). split; [| split ]. 
+
+          eapply bstep_fuel_OOT_monotonic. eapply eval_ctx_app_OOT_Ehalt. eassumption. eassumption. omega.
+
+          replace c2 with (c2 - cost (Eletapp x f' t ys e1) + cost (Eletapp x f' t ys e1)) by (simpl in *; omega). 
+          now eapply Hless_steps_letapp_OOT'; eauto.
+          simpl; eauto. 
+  Qed.
+
+  
+End Inline_correct.
+
+      
